src/Analysis/Instances/Interval/Ctx/Interval_Ctx_Call_String_Sound.thy
@@ -39,7 +39,9 @@ definition cs_call_string_eqs ::
   "cs_call_string_eqs k gs is_bot_pred Pi ps mnm main =
      side_cfg_T_eff_keyed_seed_dg_buffered intra_predecessor_addr_list (\<lambda>_. Call_String_Context.Global)
        (cs_route k)
-       (routed_cmb_g_contribution (ectx_spec gs is_bot_pred) Call_String_Context.Global Call_String_Context.Seed)
+       (routed_cmb_g_contribution (ectx_spec gs is_bot_pred)
+          Call_String_Context.Global Call_String_Context.Seed
+          (static_resolve (compile_prog Pi ps mnm main)))
        (routed_extra_g Call_String_Context.Seed Call_String_Context.Global)
        (compile_prog Pi ps mnm main) (ectx_spec gs is_bot_pred) Bot (Lifted cinit_ivl_st) Bot"
 
