src/Core/Solver/Context/DG/Call_String_Routed_Context.thy
@@ -26,7 +26,8 @@ text \<open>
 
 locale call_string_routed_context =
   dg_ctx_activation_base S gamma_dg_base gs "compile_prog Pi ps mnm main" Global "cs_route k"
-    "routed_cmb_g S Global Seed" "routed_extra_g Seed Global"
+    "routed_cmb_g S Global Seed (static_resolve (compile_prog Pi ps mnm main))"
+    "routed_extra_g Seed Global"
     bot0 s0d s0g sigma vars x0 sg gamma_state_lift
   for S :: "('a::sound_domain abs_state lifted, 'G::bounded_semilattice_sup_bot) dg_spec"
     and gs :: "vname \<Rightarrow> bool"
@@ -50,11 +51,19 @@ locale call_string_routed_context =
 begin
 
 sublocale routed: routed_context_hetero S gs "compile_prog Pi ps mnm main" Global
-  "cs_route k" bot0 s0d s0g sigma vars x0 sg Seed "cs_context k"
+  "cs_route k" bot0 s0d s0g sigma vars x0 sg Seed
+  "static_resolve (compile_prog Pi ps mnm main)" "cs_context k"
 proof unfold_locales
   show "finite (calls (compile_prog Pi ps mnm main))" using compile_prog_finite by simp
 next
   show "\<And>p ctx. Seed p ctx \<noteq> Global" by simp
+next
+  fix u ctx dst pars args p cont s
+  assume "(u, CallEdge dst pars args, FunctionEntry p, cont)
+            \<in> calls (compile_prog Pi ps mnm main)"
+  then show "p \<in> set (static_resolve (compile_prog Pi ps mnm main) cont u
+                        (CallEdge dst pars args) (locals (sigma (Inl (u, ctx)))))"
+    by (simp add: static_resolve_iff compile_prog_finite)
 next
   fix u ctx dst pars args p cont s
   show "cs_route k u ctx (enter_local S pars args (locals (sigma (Inl (u, ctx))))
