src/Core/Solver/Context/DG/Routed_Context_Unit.thy
@@ -80,7 +80,7 @@ text \<open>
 
 locale unit_routed_context =
   dg_ctx_activation_base S gammaDG gs g gk0 route_unit
-    "routed_cmb_g S gk0 seed_key" "routed_extra_g seed_key gk0"
+    "routed_cmb_g S gk0 seed_key (static_resolve g)" "routed_extra_g seed_key gk0"
     bot0 s0d s0g sigma vars x0 sg gammaM
   for S :: "('D::bounded_semilattice_sup_bot, 'G::bounded_semilattice_sup_bot) dg_spec"
     and gammaDG :: "'D \<Rightarrow> 'G \<Rightarrow> store set"
@@ -113,11 +113,17 @@ locale unit_routed_context =
 begin
 
 sublocale routed: routed_context_base_hetero S gammaDG gs g gk0 route_unit
-  bot0 s0d s0g sigma vars x0 sg seed_key gammaM enterc_unit
+  bot0 s0d s0g sigma vars x0 sg seed_key "static_resolve g" gammaM enterc_unit
 proof unfold_locales
   show "finite (calls g)" by (rule finC)
 next
   show "\<And>p ctx. seed_key p ctx \<noteq> gk0" by (rule seed_key_ne_gk0)
+next
+  fix u ctx dst pars args p cont s
+  assume "(u, CallEdge dst pars args, FunctionEntry p, cont) \<in> calls g"
+  then show "p \<in> set (static_resolve g cont u (CallEdge dst pars args)
+                        (locals (sigma (Inl (u, ctx)))))"
+    by (simp add: static_resolve_iff[OF finC])
 next
   fix u ctx dst pars args p cont s
   show "route_unit u ctx (enter_local S pars args (locals (sigma (Inl (u, ctx))))
@@ -185,11 +191,17 @@ locale unit_routed_context_hetero =
 begin
 
 sublocale hetero: routed_context_hetero S gs g gk0 route_unit
-  bot0 s0d s0g sigma vars x0 sg seed_key enterc_unit
+  bot0 s0d s0g sigma vars x0 sg seed_key "static_resolve g" enterc_unit
 proof unfold_locales
   show "finite (calls g)" by (rule finC)
 next
   show "\<And>p ctx. seed_key p ctx \<noteq> gk0" by (rule seed_key_ne_gk0)
+next
+  fix u ctx dst pars args p cont s
+  assume "(u, CallEdge dst pars args, FunctionEntry p, cont) \<in> calls g"
+  then show "p \<in> set (static_resolve g cont u (CallEdge dst pars args)
+                        (locals (sigma (Inl (u, ctx)))))"
+    by (simp add: static_resolve_iff[OF finC])
 next
   fix u ctx dst pars args p cont s
   show "route_unit u ctx (enter_local S pars args (locals (sigma (Inl (u, ctx))))
