src/Examples/Sign/CallString/Example_Sign_DG_CallString_K2.thy
@@ -26,7 +26,8 @@ definition sign_nest_2_eqs ::
      (sign exec_dg_st lifted, sign exec_dg_st lifted) dg_state) eqsT" where
   "sign_nest_2_eqs =
      side_cfg_T_eff_keyed_seed_dg intra_predecessor_addr_list (\<lambda>_. Global) (cs_route 2)
-       (routed_cmb_g sign_nest_S_st Global Seed) (routed_extra_g Seed Global)
+       (routed_cmb_g sign_nest_S_st Global Seed (static_resolve sign_nest_cfg))
+       (routed_extra_g Seed Global)
        sign_nest_cfg sign_nest_S_st Bot (Lifted cinit_sign_st) Bot"
 
 definition sign_nest_2_sol ::
@@ -136,7 +137,8 @@ abbreviation sigma_2 ::
 theorem sign_nest_2_pp_abs:
   "part_post_solution
      (side_cfg_T_eff_keyed_seed_dg intra_predecessor_addr_list (\<lambda>_. Global) (cs_route 2)
-       (routed_cmb_g sign_nest_S_abs Global Seed) (routed_extra_g Seed Global)
+       (routed_cmb_g sign_nest_S_abs Global Seed (static_resolve sign_nest_cfg))
+       (routed_extra_g Seed Global)
         sign_nest_cfg sign_nest_S_abs
         (map_lift (fun_of_resolved_st_q_for sign_nest_gs) (Bot::sign exec_dg_st lifted))
         (map_lift (fun_of_resolved_st_q_for sign_nest_gs) (Lifted cinit_sign_st))
